
> **Logistic regression‚Äôs decision boundary**  
with  
> **The general equation of a line: \( 0 = ax + by + c \)**

---

## üß† Step-by-step breakdown:

### 1Ô∏è‚É£ **Logistic regression decision function:**

In **logistic regression**, you compute:
\[
z = w \cdot x + b = w_1x_1 + w_2x_2 + \dots + w_nx_n + b
\]

This `z` is the input to the **sigmoid function**:
\[
\sigma(z) = \frac{1}{1 + e^{-z}}
\]

---

### 2Ô∏è‚É£ **Decision boundary at probability 0.5:**

Sigmoid output is **0.5** when \( z = 0 \), because:
\[
\sigma(0) = \frac{1}{1 + e^{0}} = 0.5
\]

So the **decision boundary** is when:
\[
w \cdot x + b = 0
\]

This defines the **line (or hyperplane)** that separates the classes.

---

### 3Ô∏è‚É£ **Compare to general linear equation:**

The general form of a 2D line is:
\[
0 = ax + by + c
\]

Let‚Äôs match terms:

| Logistic Regression Form | General Line Form |
|--------------------------|-------------------|
| \( w_1x_1 + w_2x_2 + b = 0 \) | \( ax + by + c = 0 \) |

So we can directly substitute:
- \( a = w_1 \)
- \( b = w_2 \)
- \( c = b \) (bias term)

‚úÖ **They are mathematically the same form!**

---

## üß© Visual Example:

If:
\[
w = [1, -1], \quad b = 0
\Rightarrow w \cdot x + b = x_1 - x_2 = 0
\Rightarrow x = y
\]

Which matches:
\[
0 = x - y
\Rightarrow a = 1, b = -1, c = 0
\]

Same as the decision boundary you showed in the original diagram!

---

### üß† Summary

- Logistic regression draws a decision boundary at:  
  \[
  w \cdot x + b = 0
  \]
- This **is equivalent** to the general linear form:
  \[
  0 = ax + by + c
  \]
- The parameters \( w_1, w_2 \) become the line's coefficients \( a, b \), and the bias becomes \( c \).

---

